Decompose specialized reasoning of memory merges
The specialized reasoning of to_partial_memory_merge_memories_* can be
seen (among other possibilities) as a quest to determine that the
domains of the two memories coincide with the domain of the two
interfaces under consideration. We can move from the hypotheses in our
proofs of simulation to that simpler assertion by a couple of simpler
results, and this transformation can further simplify either the
statement of the memory merge theorems (by slightly complicating their
appearance in the main proof) or their proof.

Co-authored-by: Florian Groult <florian.groult@inria.fr>

Intermediate/CS.v
@@ -38,6 +38,9 @@ Instance state_turn : HasTurn state := {
     Pointer.component pc \in domm iface
 }.
 
+Definition state_mem (st : state) : Memory.t :=
+  let '(_, mem, _, _) := st in mem.
+
 (* preparing the machine for running a program *)
 
 Definition initial_machine_state (p: program) : state :=
@@ -881,6 +884,11 @@ Proof.
   - subst. reflexivity.
 Qed.
 
+Remark step_preserves_mem_domm G s t s' :
+  CS.step G s t s' ->
+  domm (state_mem s) = domm (state_mem s').
+Admitted. (* Grade 1. *)
+
 Definition comes_from_initial_state (s: state) (iface : Program.interface) : Prop :=
   exists p mainP s0 t,
     well_formed_program p /\
@@ -899,5 +907,10 @@ Proof.
   rewrite <- (unionmC Hdisjoint).
   exact Hfrom_initial.
 Qed.
+
+Remark comes_from_initial_state_mem_domm s ctx :
+  comes_from_initial_state s ctx ->
+  domm (state_mem s) = domm ctx.
+Admitted. (* Grade 1. *)
 
 End CS.
